Quick reset back to old semantics.

common/Smallstep.v
@@ -26,8 +26,6 @@ Require Import Events.
 Require Import Globalenvs.
 Require Import Integers.
 
-Require Import Values. (*for meminj, compose_meminj,...*)
-
 Set Implicit Arguments.
 
 (** * Closures of transitions relations *)
@@ -474,13 +472,13 @@ End CLOSURES.
 (** * Transition semantics *)
 
 (** The general form of a transition semantics. *)
-Require Import compcert.common.Memory.
+
 Record semantics : Type := Semantics_gen {
   state: Type;
   genvtype: Type;
-  step : genvtype -> (state * mem) -> trace -> (state * mem) -> Prop;
-  initial_state: (state * mem) -> Prop;
-  final_state: (state * mem) -> int -> Prop;
+  step : genvtype -> state -> trace -> state -> Prop;
+  initial_state: state -> Prop;
+  final_state: state -> int -> Prop;
   globalenv: genvtype;
   symbolenv: Senv.t
 }.
@@ -488,9 +486,9 @@ Record semantics : Type := Semantics_gen {
 (** The form used in earlier CompCert versions, for backward compatibility. *)
 
 Definition Semantics {state funtype vartype: Type}
-                     (step: Genv.t funtype vartype -> (state * mem) -> trace -> (state * mem) -> Prop)
-                     (initial_state: (state * mem) -> Prop)
-                     (final_state: (state * mem) -> int -> Prop)
+                     (step: Genv.t funtype vartype -> state -> trace -> state -> Prop)
+                     (initial_state: state -> Prop)
+                     (final_state: state -> int -> Prop)
                      (globalenv: Genv.t funtype vartype) :=
   {| state := state;
      genvtype := Genv.t funtype vartype;
@@ -517,25 +515,20 @@ Open Scope smallstep_scope.
 
 Record fsim_properties (L1 L2: semantics) (index: Type)
                        (order: index -> index -> Prop)
-                       (match_states: index -> meminj -> (state L1 * mem) -> (state L2 * mem) -> Prop) : Prop :=
-  {
+                       (match_states: index -> state L1 -> state L2 -> Prop) : Prop := {
     fsim_order_wf: well_founded order;
-    fsim_match_meminj: forall i f s1 s2, match_states i f s1 s2 ->  Mem.inject f (snd s1) (snd s2);
-(*    fsim_match_initial_states:
-      forall s1 m1 f m2, initial_state L1 (s1,m1) -> Mem.inject f m1 m2 ->
-      exists i, exists s2, initial_state L2 (s2,m2) /\ match_states i f (s1,m1) (s2,m2);*)
     fsim_match_initial_states:
-      forall s1 m1, initial_state L1 (s1,m1) -> 
-      exists i f s2 m2, initial_state L2 (s2,m2) /\ match_states i f (s1,m1) (s2,m2) /\ Mem.inject f m1 m2;
+      forall s1, initial_state L1 s1 ->
+      exists i, exists s2, initial_state L2 s2 /\ match_states i s1 s2;
     fsim_match_final_states:
-      forall i s1 m1 s2 m2 r f,
-      match_states i f (s1,m1) (s2 ,m2) -> final_state L1 (s1,m1) r -> (final_state L2 (s2,m2) r /\ (*include this term???*) Mem.inject f m1 m2);
+      forall i s1 s2 r,
+      match_states i s1 s2 -> final_state L1 s1 r -> final_state L2 s2 r;
     fsim_simulation:
-      forall s1 t s1' f, Step L1 s1 t s1' ->
-      forall i s2, match_states i f s1 s2 ->
-      exists i', exists s2' f',
+      forall s1 t s1', Step L1 s1 t s1' ->
+      forall i s2, match_states i s1 s2 ->
+      exists i', exists s2',
          (Plus L2 s2 t s2' \/ (Star L2 s2 t s2' /\ order i' i))
-      /\ match_states i' f' s1' s2';
+      /\ match_states i' s1' s2';
     fsim_public_preserved:
       forall id, Senv.public_symbol (symbolenv L2) id = Senv.public_symbol (symbolenv L1) id
   }.
@@ -545,7 +538,7 @@ Arguments fsim_properties: clear implicits.
 Inductive forward_simulation (L1 L2: semantics) : Prop :=
   Forward_simulation (index: Type)
                      (order: index -> index -> Prop)
-                     (match_states: index -> meminj -> (state L1 * mem) -> (state L2 * mem) -> Prop)
+                     (match_states: index -> state L1 -> state L2 -> Prop)
                      (props: fsim_properties L1 L2 index order match_states).
 
 Arguments Forward_simulation {L1 L2 index} order match_states props.
@@ -554,17 +547,17 @@ Arguments Forward_simulation {L1 L2 index} order match_states props.
 
 Lemma fsim_simulation':
   forall L1 L2 index order match_states, fsim_properties L1 L2 index order match_states ->
-  forall i s1 t s1' f, Step L1 s1 t s1' ->
-  forall s2, match_states i f s1 s2 ->
-  (exists i', exists s2' f', Plus L2 s2 t s2' /\ match_states i' f' s1' s2')
-  \/ (exists i' f', order i' i /\ t = E0 /\ match_states i' f' s1' s2).
+  forall i s1 t s1', Step L1 s1 t s1' ->
+  forall s2, match_states i s1 s2 ->
+  (exists i', exists s2', Plus L2 s2 t s2' /\ match_states i' s1' s2')
+  \/ (exists i', order i' i /\ t = E0 /\ match_states i' s1' s2).
 Proof.
   intros. exploit fsim_simulation; eauto.
-  intros [i' [s2' [f' [A B]]]]. intuition.
-  left; exists i'; exists s2'; auto. exists f'; eauto.
+  intros [i' [s2' [A B]]]. intuition.
+  left; exists i'; exists s2'; auto.
   inv H3.
-  right; exists i', f'; auto.
-  left; exists i'; exists s2',f' ; split; auto. econstructor; eauto.
+  right; exists i'; auto.
+  left; exists i'; exists s2'; split; auto. econstructor; eauto.
 Qed.
 
 (** ** Forward simulation diagrams. *)
@@ -579,20 +572,17 @@ Variable L2: semantics.
 Hypothesis public_preserved:
   forall id, Senv.public_symbol (symbolenv L2) id = Senv.public_symbol (symbolenv L1) id.
 
-Variable match_states: meminj -> (state L1 * mem) -> (state L2 * mem) -> Prop.
-(*
+Variable match_states: state L1 -> state L2 -> Prop.
+
 Hypothesis match_initial_states:
-  forall s1 m1 f m2, initial_state L1 (s1,m1) -> Mem.inject f m1 m2 ->
-  exists s2, initial_state L2 (s2,m2) /\ match_states f (s1,m1) (s2,m2).*)
-Hypothesis match_initial_states:
-  forall s1 m1, initial_state L1 (s1,m1) ->
-  exists s2 f m2, initial_state L2 (s2,m2) /\ match_states f (s1,m1) (s2,m2) /\  Mem.inject f m1 m2.
+  forall s1, initial_state L1 s1 ->
+  exists s2, initial_state L2 s2 /\ match_states s1 s2.
 
 Hypothesis match_final_states:
-  forall f s1 s2 r,
-  match_states f s1 s2 ->
+  forall s1 s2 r,
+  match_states s1 s2 ->
   final_state L1 s1 r ->
-  final_state L2 s2 r  /\ Mem.inject f (snd s1) (snd s2).
+  final_state L2 s2 r.
 
 (** Simulation when one transition in the first program
     corresponds to zero, one or several transitions in the second program.
@@ -611,28 +601,21 @@ Hypothesis order_wf: well_founded order.
 
 Hypothesis simulation:
   forall s1 t s1', Step L1 s1 t s1' ->
-  forall s2 f, match_states f s1 s2 ->
-  exists s2' f',
-  (Plus L2 s2 t s2' \/ (Star L2 s2 t s2' /\ order (fst s1') (fst s1)))
-  /\ match_states f' s1' s2'.
-
-Hypothesis match_meminj : forall (f : meminj) (s1 : state L1 * mem) (s2 : state L2 * mem),
-                        match_states f s1 s2 -> Mem.inject f (snd s1) (snd s2).
+  forall s2, match_states s1 s2 ->
+  exists s2',
+  (Plus L2 s2 t s2' \/ (Star L2 s2 t s2' /\ order s1' s1))
+  /\ match_states s1' s2'.
 
 Lemma forward_simulation_star_wf: forward_simulation L1 L2.
 Proof.
-  eapply Forward_simulation with order (fun idx f s1 s2 => idx = fst s1 /\ match_states f s1 s2);
+  apply Forward_simulation with order (fun idx s1 s2 => idx = s1 /\ match_states s1 s2);
   constructor.
-  - auto.
-  - intros ? ? ? ? [? ?].
-    eapply match_meminj; eauto.
-
-  - intros. exploit match_initial_states; eauto. (*intros [s2 [A B]].
-    exists s1; exists s2; auto.*)
-    intros [s2 [f [m2 [A [B C]]]]]. exists s1; exists f; exists s2, m2; auto.
-- intros. destruct H. exploit match_final_states; eauto.
-- intros. destruct H0. subst i. exploit simulation; eauto. intros [s2' [f' [A B]]].
-  exists (fst s1'); exists s2'; exists f'; intuition auto.
+- auto.
+- intros. exploit match_initial_states; eauto. intros [s2 [A B]].
+    exists s1; exists s2; auto.
+- intros. destruct H. eapply match_final_states; eauto.
+- intros. destruct H0. subst i. exploit simulation; eauto. intros [s2' [A B]].
+  exists s1'; exists s2'; intuition auto.
 - auto.
 Qed.
 
@@ -648,21 +631,17 @@ Variable measure: state L1 -> nat.
 
 Hypothesis simulation:
   forall s1 t s1', Step L1 s1 t s1' ->
-  forall s2 f, match_states f s1 s2 -> exists f',
-  (exists s2', Plus L2 s2 t s2' /\ match_states f' s1' s2')
-  \/ (measure (fst s1') < measure (fst s1) /\ t = E0 /\ match_states f' s1' s2)%nat.
-
-Hypothesis match_meminj : forall (f : meminj) (s1 : state L1 * mem) (s2 : state L2 * mem),
-                        match_states f s1 s2 -> Mem.inject f (snd s1) (snd s2).
+  forall s2, match_states s1 s2 ->
+  (exists s2', Plus L2 s2 t s2' /\ match_states s1' s2')
+  \/ (measure s1' < measure s1 /\ t = E0 /\ match_states s1' s2)%nat.
 
 Lemma forward_simulation_star: forward_simulation L1 L2.
 Proof.
   apply forward_simulation_star_wf with (ltof _ measure).
   apply well_founded_ltof.
-  intros. exploit simulation; eauto. intros [f' [[s2' [A B]] | [A [B C]]]].
-  exists s2', f'; auto.
-  exists s2, f'; split. right; split. rewrite B. apply star_refl. auto. auto.
-  eapply match_meminj.
+  intros. exploit simulation; eauto. intros [[s2' [A B]] | [A [B C]]].
+  exists s2'; auto.
+  exists s2; split. right; split. rewrite B. apply star_refl. auto. auto.
 Qed.
 
 End SIMULATION_STAR.
@@ -674,18 +653,13 @@ Section SIMULATION_PLUS.
 
 Hypothesis simulation:
   forall s1 t s1', Step L1 s1 t s1' ->
-  forall s2 f, match_states f s1 s2 ->
-          exists s2' f', Plus L2 s2 t s2' /\ match_states f' s1' s2'.
-
-
-Hypothesis match_meminj : forall (f : meminj) (s1 : state L1 * mem) (s2 : state L2 * mem),
-                        match_states f s1 s2 -> Mem.inject f (snd s1) (snd s2).
+  forall s2, match_states s1 s2 ->
+  exists s2', Plus L2 s2 t s2' /\ match_states s1' s2'.
 
 Lemma forward_simulation_plus: forward_simulation L1 L2.
 Proof.
   apply forward_simulation_star with (measure := fun _ => O).
-  intros. exploit simulation; eauto. intros [s2' [f' [X]]]. exists f'. eauto.
-  eapply match_meminj.
+  intros. exploit simulation; eauto.
 Qed.
 
 End SIMULATION_PLUS.
@@ -697,19 +671,14 @@ Section SIMULATION_STEP.
 
 Hypothesis simulation:
   forall s1 t s1', Step L1 s1 t s1' ->
-  forall s2 f, match_states f s1 s2 ->
-          exists s2' f', Step L2 s2 t s2' /\ match_states f' s1' s2'.
-
-
-Hypothesis match_meminj : forall (f : meminj) (s1 : state L1 * mem) (s2 : state L2 * mem),
-                        match_states f s1 s2 -> Mem.inject f (snd s1) (snd s2).
+  forall s2, match_states s1 s2 ->
+  exists s2', Step L2 s2 t s2' /\ match_states s1' s2'.
 
 Lemma forward_simulation_step: forward_simulation L1 L2.
 Proof.
   apply forward_simulation_plus.
-  intros. exploit simulation; eauto. intros [s2' [f' [A B]]].
-  exists s2', f'; split; auto. apply plus_one; auto.
-  eapply match_meminj.
+  intros. exploit simulation; eauto. intros [s2' [A B]].
+  exists s2'; split; auto. apply plus_one; auto.
 Qed.
 
 End SIMULATION_STEP.
@@ -726,20 +695,16 @@ Variable measure: state L1 -> nat.
 
 Hypothesis simulation:
   forall s1 t s1', Step L1 s1 t s1' ->
-  forall s2 f, match_states f s1 s2 -> exists f',
-  (exists s2', Step L2 s2 t s2' /\ match_states f' s1' s2')
-  \/ (measure (fst s1') < measure (fst s1) /\ t = E0 /\ match_states f' s1' s2)%nat.
-
-Hypothesis match_meminj : forall (f : meminj) (s1 : state L1 * mem) (s2 : state L2 * mem),
-                        match_states f s1 s2 -> Mem.inject f (snd s1) (snd s2).
+  forall s2, match_states s1 s2 ->
+  (exists s2', Step L2 s2 t s2' /\ match_states s1' s2')
+  \/ (measure s1' < measure s1 /\ t = E0 /\ match_states s1' s2)%nat.
 
 Lemma forward_simulation_opt: forward_simulation L1 L2.
 Proof.
   apply forward_simulation_star with measure.
-  intros. exploit simulation; eauto. intros [f' [[s2' [A B]] | [A [B C]]]].
-  exists f'. left; exists s2'; split; auto. apply plus_one; auto.
-  exists f'. right; auto.
-  eapply match_meminj.
+  intros. exploit simulation; eauto. intros [[s2' [A B]] | [A [B C]]].
+  left; exists s2'; split; auto. apply plus_one; auto.
+  right; auto.
 Qed.
 
 End SIMULATION_OPT.
@@ -754,49 +719,49 @@ Context L1 L2 index order match_states (S: fsim_properties L1 L2 index order mat
 
 Lemma simulation_star:
   forall s1 t s1', Star L1 s1 t s1' ->
-  forall i f s2, match_states i f s1 s2 ->
-  exists i' f', exists s2', Star L2 s2 t s2' /\ match_states i' f' s1' s2'.
+  forall i s2, match_states i s1 s2 ->
+  exists i', exists s2', Star L2 s2 t s2' /\ match_states i' s1' s2'.
 Proof.
   induction 1; intros.
-  exists i, f; exists s2; split; auto. apply star_refl.
-  exploit fsim_simulation; eauto. intros [i' [s2' [f' [A B]]]].
-  exploit IHstar; eauto. intros [i'' [f'' [s2'' [C D]]]].
-  exists i'';exists f''; exists s2''; split; auto. eapply star_trans; eauto.
+  exists i; exists s2; split; auto. apply star_refl.
+  exploit fsim_simulation; eauto. intros [i' [s2' [A B]]].
+  exploit IHstar; eauto. intros [i'' [s2'' [C D]]].
+  exists i''; exists s2''; split; auto. eapply star_trans; eauto.
   intuition auto. apply plus_star; auto.
 Qed.
 
 Lemma simulation_plus:
   forall s1 t s1', Plus L1 s1 t s1' ->
-  forall i f s2, match_states i f s1 s2 -> 
-  (exists i', exists f', exists s2', Plus L2 s2 t s2' /\ match_states i' f' s1' s2')
-  \/ (exists i', exists f', clos_trans _ order i' i /\ t = E0 /\ match_states i' f' s1' s2).
+  forall i s2, match_states i s1 s2 ->
+  (exists i', exists s2', Plus L2 s2 t s2' /\ match_states i' s1' s2')
+  \/ (exists i', clos_trans _ order i' i /\ t = E0 /\ match_states i' s1' s2).
 Proof.
   induction 1 using plus_ind2; intros.
 (* base case *)
-  exploit fsim_simulation'; eauto. intros [[i' [s2' [f' A]]] | [i' [f' A]]].
-  left. exists i', f', s2'; auto.
-  right; exists i', f'; intuition.
+  exploit fsim_simulation'; eauto. intros [A | [i' A]].
+  left; auto.
+  right; exists i'; intuition.
 (* inductive case *)
-  exploit fsim_simulation'; eauto. intros [[i' [s2' [f' [A B]]]] | [i' [f' [A [B C]]]]].
+  exploit fsim_simulation'; eauto. intros [[i' [s2' [A B]]] | [i' [A [B C]]]].
   exploit simulation_star. apply plus_star; eauto. eauto.
-  intros [i'' [f'' [s2'' [P Q]]]].
-  left; exists i''; exists f''; exists s2''; split; auto. eapply plus_star_trans; eauto.
-  exploit IHplus; eauto. intros [[i'' [f'' [s2'' [P Q]]]] | [i'' [f'' [P [Q R]]]]].
-  subst. simpl. left; exists i''; exists f''; exists s2''; auto.
-  subst. simpl. right; exists i''; exists f''; intuition auto.
+  intros [i'' [s2'' [P Q]]].
+  left; exists i''; exists s2''; split; auto. eapply plus_star_trans; eauto.
+  exploit IHplus; eauto. intros [[i'' [s2'' [P Q]]] | [i'' [P [Q R]]]].
+  subst. simpl. left; exists i''; exists s2''; auto.
+  subst. simpl. right; exists i''; intuition auto.
   eapply t_trans; eauto. eapply t_step; eauto.
 Qed.
 
 Lemma simulation_forever_silent:
-  forall i f s1 s2,
-  Forever_silent L1 s1 -> match_states i f s1 s2 ->
+  forall i s1 s2,
+  Forever_silent L1 s1 -> match_states i s1 s2 ->
   Forever_silent L2 s2.
 Proof.
-  assert (forall i f s1 s2,
-          Forever_silent L1 s1 -> match_states i f s1 s2 ->
+  assert (forall i s1 s2,
+          Forever_silent L1 s1 -> match_states i s1 s2 ->
           forever_silent_N (step L2) order (globalenv L2) i s2).
     cofix COINDHYP; intros.
-    inv H. destruct (fsim_simulation S _ _ _ f H1 _ _ H0) as [i' [s2' [f' [A B]]]].
+    inv H. destruct (fsim_simulation S _ _ _ H1 _ _ H0) as [i' [s2' [A B]]].
     destruct A as [C | [C D]].
     eapply forever_silent_N_plus; eauto.
     eapply forever_silent_N_star; eauto.
@@ -804,13 +769,13 @@ Proof.
 Qed.
 
 Lemma simulation_forever_reactive:
-  forall i f s1 s2 T,
-  Forever_reactive L1 s1 T -> match_states i f s1 s2 ->
+  forall i s1 s2 T,
+  Forever_reactive L1 s1 T -> match_states i s1 s2 ->
   Forever_reactive L2 s2 T.
 Proof.
   cofix COINDHYP; intros.
   inv H.
-  edestruct simulation_star as [i' [f' [st2' [A B]]]]; eauto.
+  edestruct simulation_star as [i' [st2' [A B]]]; eauto.
   econstructor; eauto.
 Qed.
 
@@ -827,51 +792,35 @@ Proof.
 
   set (ff_index := (index' * index)%type).
   set (ff_order := lex_ord (clos_trans _ order') order).
-  set (ff_match_states := fun (i: ff_index) f (s1: state L1 * mem) (s3: state L3 * mem) =>
-                             exists s2 f1 f2, match_states (snd i) f1 s1 s2 /\ match_states' (fst i) f2 s2 s3 /\
-                             compose_meminj f1 f2=f).
+  set (ff_match_states := fun (i: ff_index) (s1: state L1) (s3: state L3) =>
+                             exists s2, match_states (snd i) s1 s2 /\ match_states' (fst i) s2 s3).
   apply Forward_simulation with ff_order ff_match_states; constructor.
 - (* well founded *)
   unfold ff_order. apply wf_lex_ord. apply wf_clos_trans.
   eapply fsim_order_wf; eauto. eapply fsim_order_wf; eauto.
-- (* Mem.inject *) (*The alternative def of fsim fails here*)
-  intros.
-  unfold ff_match_states in H.
-  destruct H as [s3 [f1 [f2 [MS1 [MS2 compF]]]]].
-  rewrite <- compF.
-  eapply 
-    Mem.inject_compose; first [eapply props;eassumption | eapply props';eassumption].
-- (* initial states *) (*The alternative def of fsim fails here*)
-  intros. exploit (fsim_match_initial_states props); eauto.
-  intros [i [f [s2 [m2 [A [B BB]]]]]].
-  exploit (fsim_match_initial_states props'); eauto. intros [i' [f' [s3 [m3 [C [D DD]]]]]].
-  exists (i', i), (compose_meminj f f'); exists s3, m3; split; auto.
-  split. exists (s2, m2), f, f'; auto.
-  eapply Mem.inject_compose; eauto.
+- (* initial states *)
+  intros. exploit (fsim_match_initial_states props); eauto. intros [i [s2 [A B]]].
+  exploit (fsim_match_initial_states props'); eauto. intros [i' [s3 [C D]]].
+  exists (i', i); exists s3; split; auto. exists s2; auto.
 - (* final states *)
-  intros i s1 m1 s3 m3 r f H FS1. destruct H as [[s2 m2] [f1 [f2 [A [B C]]]]].
-  assert (final_state L2 (s2, m2) r /\ Mem.inject f1 m1 m2).
-    { eapply (fsim_match_final_states props); eauto. }
-  destruct H as [FS2 INJ12].
-  assert (final_state L3 (s3, m3) r /\ Mem.inject f2 m2 m3).
-  { eapply (fsim_match_final_states props'); eauto. }
-  destruct H as [FS3 INJ23].
-  split; trivial. subst; eapply Mem.inject_compose; eauto.
+  intros. destruct H as [s3 [A B]].
+  eapply (fsim_match_final_states props'); eauto.
+  eapply (fsim_match_final_states props); eauto.
 - (* simulation *)
-  intros. rename s2 into s3. destruct H0 as [s2 [f1 [f2 [A [B C]]]]]; subst. destruct i as [i2 i1]; simpl in *.
-  exploit (fsim_simulation' props); eauto. intros [[i1' [s2' [g1 [C D]]]] | [i1' [g1 [C [D E]]]]].
+  intros. destruct H0 as [s3 [A B]]. destruct i as [i2 i1]; simpl in *.
+  exploit (fsim_simulation' props); eauto. intros [[i1' [s3' [C D]]] | [i1' [C [D E]]]].
 + (* L2 makes one or several steps. *)
-  exploit simulation_plus; eauto. intros [[i2' [g2 [s3' [P Q]]]] | [i2' [g2 [P [Q R]]]]].
+  exploit simulation_plus; eauto. intros [[i2' [s2' [P Q]]] | [i2' [P [Q R]]]].
 * (* L3 makes one or several steps *)
-  exists (i2', i1'); exists s3', (compose_meminj g1 g2); split. auto. exists s2', g1, g2; auto.
+  exists (i2', i1'); exists s2'; split. auto. exists s3'; auto.
 * (* L3 makes no step *)
-  exists (i2', i1'); exists s3, (compose_meminj g1 g2); split.
+  exists (i2', i1'); exists s2; split.
   right; split. subst t; apply star_refl. red. left. auto.
-  exists s2', g1, g2; auto.
+  exists s3'; auto.
 + (* L2 makes no step *)
-  exists (i2, i1'); exists s3, (compose_meminj g1 f2); split.
+  exists (i2, i1'); exists s2; split.
   right; split. subst t; apply star_refl. red. right. auto.
-  exists s2, g1, f2; auto.
+  exists s3; auto.
 - (* symbols *)
   intros. transitivity (Senv.public_symbol (symbolenv L2) id); eapply fsim_public_preserved; eauto.
 Qed.
@@ -945,10 +894,10 @@ Proof.
 Qed.
 
 End DETERMINACY.
- 
+
 (** * Backward simulations between two transition semantics. *)
 
-Definition safe (L: semantics) (s: state L * mem) : Prop :=
+Definition safe (L: semantics) (s: state L) : Prop :=
   forall s',
   Star L s E0 s' ->
   (exists r, final_state L s' r)
@@ -965,28 +914,28 @@ Qed.
 
 Record bsim_properties (L1 L2: semantics) (index: Type)
                        (order: index -> index -> Prop)
-                       (match_states: index -> meminj -> state L1 * mem -> state L2 * mem -> Prop) : Prop := {
+                       (match_states: index -> state L1 -> state L2 -> Prop) : Prop := {
     bsim_order_wf: well_founded order;
     bsim_initial_states_exist:
       forall s1, initial_state L1 s1 -> exists s2, initial_state L2 s2;
     bsim_match_initial_states:
       forall s1 s2, initial_state L1 s1 -> initial_state L2 s2 ->
-      exists i, exists s1', exists f, initial_state L1 s1' /\ match_states i f s1' s2 /\ Mem.inject f (snd s1') (snd s2);
+      exists i, exists s1', initial_state L1 s1' /\ match_states i s1' s2;
     bsim_match_final_states:
-      forall i s1 s2 r f,
-      match_states i f s1 s2 -> safe L1 s1 -> final_state L2 s2 r ->
+      forall i s1 s2 r,
+      match_states i s1 s2 -> safe L1 s1 -> final_state L2 s2 r ->
       exists s1', Star L1 s1 E0 s1' /\ final_state L1 s1' r;
     bsim_progress:
-      forall i s1 s2 f,
-      match_states i f s1 s2 -> safe L1 s1 ->
+      forall i s1 s2,
+      match_states i s1 s2 -> safe L1 s1 ->
       (exists r, final_state L2 s2 r) \/
       (exists t, exists s2', Step L2 s2 t s2');
     bsim_simulation:
       forall s2 t s2', Step L2 s2 t s2' ->
-      forall i s1 f, match_states i f s1 s2 -> safe L1 s1 ->
-      exists i', exists f', exists s1',
+      forall i s1, match_states i s1 s2 -> safe L1 s1 ->
+      exists i', exists s1',
          (Plus L1 s1 t s1' \/ (Star L1 s1 t s1' /\ order i' i))
-      /\ match_states i' f' s1' s2';
+      /\ match_states i' s1' s2';
     bsim_public_preserved:
       forall id, Senv.public_symbol (symbolenv L2) id = Senv.public_symbol (symbolenv L1) id
   }.
@@ -996,7 +945,7 @@ Arguments bsim_properties: clear implicits.
 Inductive backward_simulation (L1 L2: semantics) : Prop :=
   Backward_simulation (index: Type)
                       (order: index -> index -> Prop)
-                      (match_states: index -> meminj -> state L1 * mem -> state L2 * mem -> Prop)
+                      (match_states: index -> state L1 -> state L2 -> Prop)
                       (props: bsim_properties L1 L2 index order match_states).
 
 Arguments Backward_simulation {L1 L2 index} order match_states props.
@@ -1006,16 +955,16 @@ Arguments Backward_simulation {L1 L2 index} order match_states props.
 Lemma bsim_simulation':
   forall L1 L2 index order match_states, bsim_properties L1 L2 index order match_states ->
   forall i s2 t s2', Step L2 s2 t s2' ->
-  forall f s1, match_states i f s1 s2 -> safe L1 s1 -> 
-  (exists i', exists s1', exists f',Plus L1 s1 t s1' /\ match_states i' f' s1' s2')
-  \/ (exists i', exists f', order i' i /\ t = E0 /\ match_states i' f' s1 s2').
+  forall s1, match_states i s1 s2 -> safe L1 s1 ->
+  (exists i', exists s1', Plus L1 s1 t s1' /\ match_states i' s1' s2')
+  \/ (exists i', order i' i /\ t = E0 /\ match_states i' s1 s2').
 Proof.
   intros. exploit bsim_simulation; eauto.
-  intros [i' [f' [s1' [A B]]]]. intuition.
-  left; exists i'; exists s1', f'; auto.
+  intros [i' [s1' [A B]]]. intuition.
+  left; exists i'; exists s1'; auto.
   inv H4.
-  right; exists i', f'; auto.
-  left; exists i'; exists s1', f'; split; auto. econstructor; eauto.
+  right; exists i'; auto.
+  left; exists i'; exists s1'; split; auto. econstructor; eauto.
 Qed.
 
 (** ** Backward simulation diagrams. *)
@@ -1030,22 +979,22 @@ Variable L2: semantics.
 Hypothesis public_preserved:
   forall id, Senv.public_symbol (symbolenv L2) id = Senv.public_symbol (symbolenv L1) id.
 
-Variable match_states: meminj -> state L1 * mem -> state L2 * mem -> Prop.
+Variable match_states: state L1 -> state L2 -> Prop.
 
 Hypothesis initial_states_exist:
   forall s1, initial_state L1 s1 -> exists s2, initial_state L2 s2.
 
 Hypothesis match_initial_states:
   forall s1 s2, initial_state L1 s1 -> initial_state L2 s2 ->
-  exists s1' f, initial_state L1 s1' /\ match_states f s1' s2 /\ Mem.inject f (snd s1') (snd s2).
+  exists s1', initial_state L1 s1' /\ match_states s1' s2.
 
 Hypothesis match_final_states:
-  forall s1 s2 r f,
-  match_states f s1 s2 -> final_state L2 s2 r -> final_state L1 s1 r /\ (*include this term???*) Mem.inject f (snd s1) (snd s2).
+  forall s1 s2 r,
+  match_states s1 s2 -> final_state L2 s2 r -> final_state L1 s1 r.
 
 Hypothesis progress:
-  forall s1 s2 f,
-  match_states f s1 s2 -> safe L1 s1 ->
+  forall s1 s2,
+  match_states s1 s2 -> safe L1 s1 ->
   (exists r, final_state L2 s2 r) \/
   (exists t, exists s2', Step L2 s2 t s2').
 
@@ -1053,20 +1002,20 @@ Section BACKWARD_SIMULATION_PLUS.
 
 Hypothesis simulation:
   forall s2 t s2', Step L2 s2 t s2' ->
-  forall s1 f, match_states f s1 s2 -> safe L1 s1 ->
-  exists s1' f', Plus L1 s1 t s1' /\ match_states f' s1' s2'.
+  forall s1, match_states s1 s2 -> safe L1 s1 ->
+  exists s1', Plus L1 s1 t s1' /\ match_states s1' s2'.
 
 Lemma backward_simulation_plus: backward_simulation L1 L2.
 Proof.
   apply Backward_simulation with
     (fun (x y: unit) => False)
-    (fun (i: unit) f s1 s2 => match_states f s1 s2);
+    (fun (i: unit) s1 s2 => match_states s1 s2);
   constructor; auto.
 - red; intros; constructor; intros. contradiction.
 - intros. exists tt; eauto.
-- intros. exists s1; split. apply star_refl. eapply match_final_states; eauto.
-- intros. exploit simulation; eauto. intros [s1' [f' [A B]]].
-  exists tt; exists f'; exists s1'; auto.
+- intros. exists s1; split. apply star_refl. eauto.
+- intros. exploit simulation; eauto. intros [s1' [A B]].
+  exists tt; exists s1'; auto.
 Qed.
 
 End BACKWARD_SIMULATION_PLUS.
@@ -1081,48 +1030,48 @@ Context L1 L2 index order match_states (S: bsim_properties L1 L2 index order mat
 
 Lemma bsim_E0_star:
   forall s2 s2', Star L2 s2 E0 s2' ->
-  forall i s1 f, match_states i f s1 s2 -> safe L1 s1 ->
-  exists i', exists s1' f', Star L1 s1 E0 s1' /\ match_states i' f' s1' s2'.
+  forall i s1, match_states i s1 s2 -> safe L1 s1 ->
+  exists i', exists s1', Star L1 s1 E0 s1' /\ match_states i' s1' s2'.
 Proof.
   intros s20 s20' STAR0. pattern s20, s20'. eapply star_E0_ind; eauto.
 - (* base case *)
-  intros. exists i; exists s1, f; split; auto. apply star_refl.
+  intros. exists i; exists s1; split; auto. apply star_refl.
 - (* inductive case *)
-  intros. exploit bsim_simulation; eauto. intros [i' [f' [s1' [A B]]]].
+  intros. exploit bsim_simulation; eauto. intros [i' [s1' [A B]]].
   assert (Star L1 s0 E0 s1'). intuition. apply plus_star; auto.
-  exploit H0. eauto. eapply star_safe; eauto. intros [i'' [s1'' [f'' [C D]]]].
-  exists i''; exists s1'', f''; split; auto. eapply star_trans; eauto.
+  exploit H0. eauto. eapply star_safe; eauto. intros [i'' [s1'' [C D]]].
+  exists i''; exists s1''; split; auto. eapply star_trans; eauto.
 Qed.
 
 Lemma bsim_safe:
-  forall i s1 s2 f,
-  match_states i f s1 s2 -> safe L1 s1 -> safe L2 s2.
+  forall i s1 s2,
+  match_states i s1 s2 -> safe L1 s1 -> safe L2 s2.
 Proof.
   intros; red; intros.
-  exploit bsim_E0_star; eauto. intros [i' [s1' [f' [A B]]]].
+  exploit bsim_E0_star; eauto. intros [i' [s1' [A B]]].
   eapply bsim_progress; eauto. eapply star_safe; eauto.
 Qed.
 
 Lemma bsim_E0_plus:
   forall s2 t s2', Plus L2 s2 t s2' -> t = E0 ->
-  forall i s1 f, match_states i f s1 s2 -> safe L1 s1 ->
-     (exists i' f', exists s1', Plus L1 s1 E0 s1' /\ match_states i' f' s1' s2')
-  \/ (exists i' f', clos_trans _ order i' i /\ match_states i' f' s1 s2').
+  forall i s1, match_states i s1 s2 -> safe L1 s1 ->
+     (exists i', exists s1', Plus L1 s1 E0 s1' /\ match_states i' s1' s2')
+  \/ (exists i', clos_trans _ order i' i /\ match_states i' s1 s2').
 Proof.
   induction 1 using plus_ind2; intros; subst t.
 - (* base case *)
-  exploit bsim_simulation'; eauto. intros [[i' [s1' [f' [A B]]]] | [i' [f' [A [B C]]]]].
-+ left; exists i', f'; exists s1'; auto.
-+ right; exists i', f'; intuition.
+  exploit bsim_simulation'; eauto. intros [[i' [s1' [A B]]] | [i' [A [B C]]]].
++ left; exists i'; exists s1'; auto.
++ right; exists i'; intuition.
 - (* inductive case *)
   exploit Eapp_E0_inv; eauto. intros [EQ1 EQ2]; subst.
-  exploit bsim_simulation'; eauto. intros [[i' [s1' [f' [A B]]]] | [i' [f' [A [B C]]]]].
+  exploit bsim_simulation'; eauto. intros [[i' [s1' [A B]]] | [i' [A [B C]]]].
 + exploit bsim_E0_star. apply plus_star; eauto. eauto. eapply star_safe; eauto. apply plus_star; auto.
-  intros [i'' [s1'' [f'' [P Q]]]].
-  left; exists i'', f''; exists s1''; intuition. eapply plus_star_trans; eauto.
-+ exploit IHplus; eauto. intros [P | [i'' [f'' [P Q]]]].
+  intros [i'' [s1'' [P Q]]].
+  left; exists i''; exists s1''; intuition. eapply plus_star_trans; eauto.
++ exploit IHplus; eauto. intros [P | [i'' [P Q]]].
   left; auto.
-  right; exists i'', f''; intuition. eapply t_trans; eauto. apply t_step; auto.
+  right; exists i''; intuition. eapply t_trans; eauto. apply t_step; auto.
 Qed.
 
 Lemma star_non_E0_split:
@@ -1158,29 +1107,28 @@ Let bb_index : Type := (index * index')%type.
 
 Definition bb_order : bb_index -> bb_index -> Prop := lex_ord (clos_trans _ order) order'.
 
-Inductive bb_match_states: bb_index -> meminj -> state L1 * mem -> state L3 * mem -> Prop :=
-  | bb_match_later: forall i1 i2 f s1 s3 s2x s2y f1 f2,
-      match_states i1 f1 s1 s2x -> Star L2 s2x E0 s2y -> match_states' i2 f2 s2y s3 ->
-      compose_meminj f1 f2=f ->
-      bb_match_states (i1, i2) f s1 s3.
+Inductive bb_match_states: bb_index -> state L1 -> state L3 -> Prop :=
+  | bb_match_later: forall i1 i2 s1 s3 s2x s2y,
+      match_states i1 s1 s2x -> Star L2 s2x E0 s2y -> match_states' i2 s2y s3 ->
+      bb_match_states (i1, i2) s1 s3.
 
-Lemma bb_match_at: forall i1 i2 s1 s3 s2 f1 f2,
-  match_states i1 f1 s1 s2 -> match_states' i2 f2 s2 s3 ->
-  bb_match_states (i1, i2) (compose_meminj f1 f2) s1 s3.
+Lemma bb_match_at: forall i1 i2 s1 s3 s2,
+  match_states i1 s1 s2 -> match_states' i2 s2 s3 ->
+  bb_match_states (i1, i2) s1 s3.
 Proof.
   intros. econstructor; eauto. apply star_refl.
 Qed.
 
 Lemma bb_simulation_base:
   forall s3 t s3', Step L3 s3 t s3' ->
-  forall i1 s1 i2 s2 f1 f2, match_states i1 f1 s1 s2 -> match_states' i2 f2 s2 s3 -> safe L1 s1 ->
-  exists i', exists s1', exists f',
+  forall i1 s1 i2 s2, match_states i1 s1 s2 -> match_states' i2 s2 s3 -> safe L1 s1 ->
+  exists i', exists s1',
     (Plus L1 s1 t s1' \/ (Star L1 s1 t s1' /\ bb_order i' (i1, i2)))
-    /\ bb_match_states i' f' s1' s3'.
+    /\ bb_match_states i' s1' s3'.
 Proof.
   intros.
   exploit (bsim_simulation' S23); eauto. eapply bsim_safe; eauto.
-  intros [ [i2' [s2' [f2' [PLUS2 MATCH2]]]] | [i2' [f2' [ORD2 [EQ MATCH2]]]]].
+  intros [ [i2' [s2' [PLUS2 MATCH2]]] | [i2' [ORD2 [EQ MATCH2]]]].
 - (* 1 L2 makes one or several transitions *)
   assert (EITHER: t = E0 \/ (length t = 1)%nat).
   { exploit L3_single_events; eauto.
@@ -1188,33 +1136,33 @@ Proof.
   destruct EITHER.
 + (* 1.1 these are silent transitions *)
   subst t. exploit (bsim_E0_plus S12); eauto.
-  intros [ [i1' [f1' [s1' [PLUS1 MATCH1]]]] | [i1' [f1' [ORD1 MATCH1]]]].
+  intros [ [i1' [s1' [PLUS1 MATCH1]]] | [i1' [ORD1 MATCH1]]].
 * (* 1.1.1 L1 makes one or several transitions *)
-  exists (i1', i2'); exists s1', (compose_meminj f1' f2'); split. auto. eapply bb_match_at; eauto.
+  exists (i1', i2'); exists s1'; split. auto. eapply bb_match_at; eauto.
 * (* 1.1.2 L1 makes no transitions *)
-  exists (i1', i2'); exists s1, (compose_meminj f1' f2'); split.
+  exists (i1', i2'); exists s1; split.
   right; split. apply star_refl. left; auto.
   eapply bb_match_at; eauto.
 + (* 1.2 non-silent transitions *)
   exploit star_non_E0_split. apply plus_star; eauto. auto.
   intros [s2x [s2y [P [Q R]]]].
-  exploit (bsim_E0_star S12). eexact P. eauto. auto. intros [i1' [s1x [g1 [X Y]]]].
+  exploit (bsim_E0_star S12). eexact P. eauto. auto. intros [i1' [s1x [X Y]]].
   exploit (bsim_simulation' S12). eexact Q. eauto. eapply star_safe; eauto.
-  intros [[i1'' [s1y [g1'' [U V]]]] | [i1'' [g1'' [U [V W]]]]]; try (subst t; discriminate).
-  exists (i1'', i2'); exists s1y. exists (compose_meminj g1'' f2'). split.
+  intros [[i1'' [s1y [U V]]] | [i1'' [U [V W]]]]; try (subst t; discriminate).
+  exists (i1'', i2'); exists s1y; split.
   left. eapply star_plus_trans; eauto. eapply bb_match_later; eauto.
 - (* 2. L2 makes no transitions *)
-  subst. exists (i1, i2'); exists s1, (compose_meminj f1 f2'); split.
+  subst. exists (i1, i2'); exists s1; split.
   right; split. apply star_refl. right; auto.
   eapply bb_match_at; eauto.
 Qed.
 
 Lemma bb_simulation:
   forall s3 t s3', Step L3 s3 t s3' ->
-  forall i s1 f, bb_match_states i f s1 s3 -> safe L1 s1 ->
-  exists i', exists s1', exists f',
+  forall i s1, bb_match_states i s1 s3 -> safe L1 s1 ->
+  exists i', exists s1',
     (Plus L1 s1 t s1' \/ (Star L1 s1 t s1' /\ bb_order i' i))
-    /\ bb_match_states i' f' s1' s3'.
+    /\ bb_match_states i' s1' s3'.
 Proof.
   intros. inv H0.
   exploit star_inv; eauto. intros [[EQ1 EQ2] | PLUS].
@@ -1222,19 +1170,19 @@ Proof.
   subst. eapply bb_simulation_base; eauto.
 - (* 2. match later *)
   exploit (bsim_E0_plus S12); eauto.
-  intros [[i1' [f1' [s1' [A B]]]] | [i1' [f1' [A B]]]].
+  intros [[i1' [s1' [A B]]] | [i1' [A B]]].
 + (* 2.1 one or several silent transitions *)
   exploit bb_simulation_base. eauto. auto. eexact B. eauto.
     eapply star_safe; eauto. eapply plus_star; eauto.
-  intros [i'' [s1'' [f'' [C D]]]].
-  exists i''; exists s1'', f''; split; auto.
+  intros [i'' [s1'' [C D]]].
+  exists i''; exists s1''; split; auto.
   left. eapply plus_star_trans; eauto.
   destruct C as [P | [P Q]]. apply plus_star; eauto. eauto.
   traceEq.
 + (* 2.2 no silent transition *)
   exploit bb_simulation_base. eauto. auto. eexact B. eauto. auto.
-  intros [i'' [s1'' [f'' [C D]]]].
-  exists i''; exists s1'', f''; split; auto.
+  intros [i'' [s1'' [C D]]].
+  exists i''; exists s1''; split; auto.
   intuition. right; intuition.
   inv H6. left. eapply t_trans; eauto. left; auto.
 Qed.
@@ -1259,27 +1207,24 @@ Proof.
 - (* match initial states *)
   intros s1 s3 INIT1 INIT3.
   exploit (bsim_initial_states_exist props); eauto. intros [s2 INIT2].
-  exploit (bsim_match_initial_states props'); eauto. intros [i2 [s2' [f2 [INIT2' M2]]]].
-  exploit (bsim_match_initial_states props); eauto. intros [i1 [s1' [f1 [INIT1' M1]]]].
-  exists (i1, i2); exists s1', (compose_meminj f1 f2); intuition auto. eapply bb_match_at; eauto.
-  eapply Mem.inject_compose; eauto.
+  exploit (bsim_match_initial_states props'); eauto. intros [i2 [s2' [INIT2' M2]]].
+  exploit (bsim_match_initial_states props); eauto. intros [i1 [s1' [INIT1' M1]]].
+  exists (i1, i2); exists s1'; intuition auto. eapply bb_match_at; eauto.
 - (* match final states *)
-  intros i s1 s3 r f MS SAFE FIN. inv MS.
+  intros i s1 s3 r MS SAFE FIN. inv MS.
   exploit (bsim_match_final_states props'); eauto.
     eapply star_safe; eauto. eapply bsim_safe; eauto.
   intros [s2' [A B]].
   exploit (bsim_E0_star props). eapply star_trans. eexact H0. eexact A. auto. eauto. auto.
-  intros [i1' [s1' [f [C D]]]].
+  intros [i1' [s1' [C D]]].
   exploit (bsim_match_final_states props); eauto. eapply star_safe; eauto.
   intros [s1'' [P Q]].
   exists s1''; split; auto. eapply star_trans; eauto.
 - (* progress *)
-  intros i s1 s3 f MS SAFE. inv MS.
+  intros i s1 s3 MS SAFE. inv MS.
   eapply (bsim_progress props'). eauto. eapply star_safe; eauto. eapply bsim_safe; eauto.
 - (* simulation *)
-  intros s3 t s3'; intros.
-  destruct (@bb_simulation L1 L2 _ L3single _ _ _ props _ _ _ props' _ _ _ H _ _ _ H0 H1)
-  as [i' [s1' [f' A]]]. exists i', f', s1'; assumption.
+  apply bb_simulation; auto.
 - (* symbols *)
   intros. transitivity (Senv.public_symbol (symbolenv L2) id); eapply bsim_public_preserved; eauto.
 Qed.
@@ -1294,33 +1239,33 @@ Hypothesis L2_determinate: determinate L2.
 
 (** Exploiting forward simulation *)
 
-Inductive f2b_transitions: state L1 * mem -> state L2 * mem -> Prop :=
+Inductive f2b_transitions: state L1 -> state L2 -> Prop :=
   | f2b_trans_final: forall s1 s2 s1' r,
       Star L1 s1 E0 s1' ->
       final_state L1 s1' r ->
       final_state L2 s2 r ->
       f2b_transitions s1 s2
-  | f2b_trans_step: forall s1 s2 s1' t s1'' s2' i' i'' f' f'',
+  | f2b_trans_step: forall s1 s2 s1' t s1'' s2' i' i'',
       Star L1 s1 E0 s1' ->
       Step L1 s1' t s1'' ->
       Plus L2 s2 t s2' ->
-      match_states i' f' s1' s2 ->
-      match_states i'' f'' s1'' s2' ->
+      match_states i' s1' s2 ->
+      match_states i'' s1'' s2' ->
       f2b_transitions s1 s2.
 
 Lemma f2b_progress:
-  forall i f s1 s2, match_states i f s1 s2 -> safe L1 s1 -> f2b_transitions s1 s2.
+  forall i s1 s2, match_states i s1 s2 -> safe L1 s1 -> f2b_transitions s1 s2.
 Proof.
   intros i0; pattern i0. apply well_founded_ind with (R := order).
   eapply fsim_order_wf; eauto.
-  intros i REC f s1 s2 MATCH SAFE.
+  intros i REC s1 s2 MATCH SAFE.
   destruct (SAFE s1) as [[r FINAL] | [t [s1' STEP1]]]. apply star_refl.
 - (* final state reached *)
   eapply f2b_trans_final; eauto.
-  apply star_refl. destruct s1 as [s1 m1]. destruct s2 as [s2 m2].
-  exploit fsim_match_final_states. apply FS. apply MATCH. simpl; apply FINAL. intros X; apply X.
+  apply star_refl.
+  eapply fsim_match_final_states; eauto.
 - (* L1 can make one step *)
-  exploit (fsim_simulation FS); eauto. intros [i' [s2' [f2' [A MATCH']]]].
+  exploit (fsim_simulation FS); eauto. intros [i' [s2' [A MATCH']]].
   assert (B: Plus L2 s2 t s2' \/ (s2' = s2 /\ t = E0 /\ order i' i)).
     intuition auto.
     destruct (star_inv H0); intuition auto.
@@ -1334,11 +1279,11 @@ Qed.
 
 Lemma fsim_simulation_not_E0:
   forall s1 t s1', Step L1 s1 t s1' -> t <> E0 ->
-  forall i s2 f, match_states i f s1 s2 ->
-  exists i', exists s2' f', Plus L2 s2 t s2' /\ match_states i' f' s1' s2'.
+  forall i s2, match_states i s1 s2 ->
+  exists i', exists s2', Plus L2 s2 t s2' /\ match_states i' s1' s2'.
 Proof.
-  intros. exploit (fsim_simulation FS); eauto. intros [i' [s2' [f2 [A B]]]].
-  exists i'; exists s2', f2; split; auto.
+  intros. exploit (fsim_simulation FS); eauto. intros [i' [s2' [A B]]].
+  exists i'; exists s2'; split; auto.
   destruct A. auto. destruct H2. exploit star_inv; eauto. intros [[EQ1 EQ2] | P]; auto.
   congruence.
 Qed.
@@ -1422,26 +1367,26 @@ Qed.
 
 (** Constructing the backward simulation *)
 
-Inductive f2b_match_states: f2b_index -> (*omit???*)meminj -> state L1 * mem -> state L2 * mem -> Prop :=
-  | f2b_match_at: forall i s1 s2 f,
-      match_states i f s1 s2 ->
-      f2b_match_states (F2BI_after O) f s1 s2
-  | f2b_match_before: forall s1 t s1' s2b s2 n s2a i f,
+Inductive f2b_match_states: f2b_index -> state L1 -> state L2 -> Prop :=
+  | f2b_match_at: forall i s1 s2,
+      match_states i s1 s2 ->
+      f2b_match_states (F2BI_after O) s1 s2
+  | f2b_match_before: forall s1 t s1' s2b s2 n s2a i,
       Step L1 s1 t s1' ->  t <> E0 ->
       Star L2 s2b E0 s2 ->
       starN (step L2) (globalenv L2) n s2 t s2a ->
-      match_states i f s1 s2b ->
-      f2b_match_states (F2BI_before n) f s1 s2
-  | f2b_match_after: forall n s2 s2a s1 i f,
+      match_states i s1 s2b ->
+      f2b_match_states (F2BI_before n) s1 s2
+  | f2b_match_after: forall n s2 s2a s1 i,
       starN (step L2) (globalenv L2) (S n) s2 E0 s2a ->
-      match_states i f s1 s2a ->
-      f2b_match_states (F2BI_after (S n)) f s1 s2.
+      match_states i s1 s2a ->
+      f2b_match_states (F2BI_after (S n)) s1 s2.
 
 Remark f2b_match_after':
-  forall n s2 s2a s1 i f,
+  forall n s2 s2a s1 i,
   starN (step L2) (globalenv L2) n s2 E0 s2a ->
-  match_states i f s1 s2a ->
-  f2b_match_states (F2BI_after n) f s1 s2.
+  match_states i s1 s2a ->
+  f2b_match_states (F2BI_after n) s1 s2.
 Proof.
   intros. inv H.
   econstructor; eauto.
@@ -1452,12 +1397,12 @@ Qed.
 
 Lemma f2b_simulation_step:
   forall s2 t s2', Step L2 s2 t s2' ->
-  forall i s1 f, f2b_match_states i f s1 s2 -> safe L1 s1 ->
-  exists i', exists s1' f',
+  forall i s1, f2b_match_states i s1 s2 -> safe L1 s1 ->
+  exists i', exists s1',
     (Plus L1 s1 t s1' \/ (Star L1 s1 t s1' /\ f2b_order i' i))
-     /\ f2b_match_states i' f' s1' s2'.
+     /\ f2b_match_states i' s1' s2'.
 Proof.
-  intros s2 t s2' STEP2 i s1 f MATCH SAFE.
+  intros s2 t s2' STEP2 i s1 MATCH SAFE.
   inv MATCH.
 - (* 1. At matching states *)
   exploit f2b_progress; eauto. intros TRANS; inv TRANS.
@@ -1471,12 +1416,12 @@ Proof.
   destruct (silent_or_not_silent t2).
   (* 1.2.1.1  L1 makes a silent transition too: perform transition now and go to "after" state *)
   subst. simpl in *. destruct (star_starN H6) as [n STEPS2].
-  exists (F2BI_after n); exists s1''; eexists. split.
+  exists (F2BI_after n); exists s1''; split.
   left. eapply plus_right; eauto.
   eapply f2b_match_after'; eauto.
   (* 1.2.1.2 L1 makes a non-silent transition: keep it for later and go to "before" state *)
   subst. simpl in *. destruct (star_starN H6) as [n STEPS2].
-  exists (F2BI_before n); exists s1'; eexists; split.
+  exists (F2BI_before n); exists s1'; split.
   right; split. auto. constructor.
   econstructor. eauto. auto. apply star_one; eauto. eauto. eauto.
 * (* 1.2.2 L2 makes a non-silent transition, and so does L1 *)
@@ -1486,7 +1431,7 @@ Proof.
   (* Use receptiveness to equate the traces *)
   exploit (sr_receptive L1_receptive); eauto. intros [s1''' STEP1].
   exploit fsim_simulation_not_E0. eexact STEP1. auto. eauto.
-  intros [i''' [s2''' [f''' [P Q]]]]. inv P.
+  intros [i''' [s2''' [P Q]]]. inv P.
   (* Exploit determinacy *)
   exploit not_silent_length. eapply (sr_traces L1_receptive); eauto. intros [EQ | EQ].
   subst t0. simpl in *. exploit sd_determ_1. eauto. eexact STEP2. eexact H2.
@@ -1494,7 +1439,7 @@ Proof.
   subst t2. rewrite E0_right in *.
   assert (s4 = s2'). eapply sd_determ_2; eauto. subst s4.
   (* Perform transition now and go to "after" state *)
-  destruct (star_starN H7) as [n STEPS2]. exists (F2BI_after n); exists s1'''; eexists; split.
+  destruct (star_starN H7) as [n STEPS2]. exists (F2BI_after n); exists s1'''; split.
   left. eapply plus_right; eauto.
   eapply f2b_match_after'; eauto.
 
@@ -1503,7 +1448,7 @@ Proof.
   exploit f2b_determinacy_inv. eexact H4. eexact STEP2.
   intros [[EQ1 [EQ2 EQ3]] | [NOT1 [NOT2 MT]]].
 + (* 2.1 L2 makes a silent transition: remain in "before" state *)
-  subst. simpl in *. exists (F2BI_before n0); exists s1; eexists; split.
+  subst. simpl in *. exists (F2BI_before n0); exists s1; split.
   right; split. apply star_refl. constructor. omega.
   econstructor; eauto. eapply star_right; eauto.
 + (* 2.2 L2 make a non-silent transition *)
@@ -1513,7 +1458,7 @@ Proof.
   (* Use receptiveness to equate the traces *)
   exploit (sr_receptive L1_receptive); eauto. intros [s1''' STEP1].
   exploit fsim_simulation_not_E0. eexact STEP1. auto. eauto.
-  intros [i''' [s2''' [f''' [P Q]]]].
+  intros [i''' [s2''' [P Q]]].
   (* Exploit determinacy *)
   exploit f2b_determinacy_star. eauto. eexact STEP2. auto. apply plus_star; eauto.
   intro R. inv R. congruence.
@@ -1523,7 +1468,7 @@ Proof.
   subst. rewrite E0_right in *.
   assert (s3 = s2'). eapply sd_determ_2; eauto. subst s3.
   (* Perform transition now and go to "after" state *)
-  destruct (star_starN H6) as [n STEPS2]. exists (F2BI_after n); exists s1'''; eexists; split.
+  destruct (star_starN H6) as [n STEPS2]. exists (F2BI_after n); exists s1'''; split.
   left. apply plus_one; auto.
   eapply f2b_match_after'; eauto.
 
@@ -1531,7 +1476,7 @@ Proof.
   inv H. exploit Eapp_E0_inv; eauto. intros [EQ1 EQ2]; subst.
   exploit f2b_determinacy_inv. eexact H2. eexact STEP2.
   intros [[EQ1 [EQ2 EQ3]] | [NOT1 [NOT2 MT]]].
-  subst. exists (F2BI_after n); exists s1; eexists; split.
+  subst. exists (F2BI_after n); exists s1; split.
   right; split. apply star_refl. constructor; omega.
   eapply f2b_match_after'; eauto.
   congruence.
@@ -1552,12 +1497,12 @@ Proof.
 - (* well founded *)
   apply wf_f2b_order.
 - (* initial states exist *)
-  intros [s1 m1] H. exploit (fsim_match_initial_states FS); eauto. intros [i [f [s2 [m2 [A [B C]]]]]].
-  exists (s2,m2); auto.
+  intros. exploit (fsim_match_initial_states FS); eauto. intros [i [s2 [A B]]].
+  exists s2; auto.
 - (* initial states *)
-  intros. destruct s1 as [s1 m1]. destruct s2 as [s2 m2]. exploit (fsim_match_initial_states FS); eauto. intros [i [f [s2' [m2' [A [B C]]]]]].
-  assert ((s2,m2) = (s2',m2')) by (eapply sd_initial_determ; eauto). inv H1. (* subst s2'.*)
-  exists (F2BI_after O); exists (s1, m1); eexists; split; auto. split. econstructor; eauto. simpl; trivial.
+  intros. exploit (fsim_match_initial_states FS); eauto. intros [i [s2' [A B]]].
+  assert (s2 = s2') by (eapply sd_initial_determ; eauto). subst s2'.
+  exists (F2BI_after O); exists s1; split; auto. econstructor; eauto.
 - (* final states *)
   intros. inv H.
   exploit f2b_progress; eauto. intros TRANS; inv TRANS.
@@ -1574,9 +1519,7 @@ Proof.
   inv H4. congruence. right; econstructor; econstructor; eauto.
   inv H1. right; econstructor; econstructor; eauto.
 - (* simulation *)
-  intros. destruct (f2b_simulation_step FS L1_receptive L2_determinate _ _ H H0 H1)
-  as [i' [s1' [f' A]]]. exists i', f', s1'; trivial. 
-  (*eapply f2b_simulation_step; eauto.*)
+  eapply f2b_simulation_step; eauto.
 - (* symbols preserved *)
   exact (fsim_public_preserved FS).
 Qed.
@@ -1593,23 +1536,23 @@ Variable L: semantics.
 
 Hypothesis Lwb: well_behaved_traces L.
 
-Inductive atomic_step (ge: genvtype L): (trace * state L * mem) -> trace -> (trace * state L * mem) -> Prop :=
-  | atomic_step_silent: forall s s' m m',
-      Step L (s,m) E0 (s',m') ->
-      atomic_step ge (E0, s, m) E0 (E0, s', m')
-  | atomic_step_start: forall s ev t s' m m',
-      Step L (s,m) (ev :: t) (s',m') ->
-      atomic_step ge (E0, s, m) (ev :: nil) (t, s', m')
-  | atomic_step_continue: forall ev t s m,
+Inductive atomic_step (ge: genvtype L): (trace * state L) -> trace -> (trace * state L) -> Prop :=
+  | atomic_step_silent: forall s s',
+      Step L s E0 s' ->
+      atomic_step ge (E0, s) E0 (E0, s')
+  | atomic_step_start: forall s ev t s',
+      Step L s (ev :: t) s' ->
+      atomic_step ge (E0, s) (ev :: nil) (t, s')
+  | atomic_step_continue: forall ev t s,
       output_trace (ev :: t) ->
-      atomic_step ge (ev :: t, s, m) (ev :: nil) (t, s, m).
+      atomic_step ge (ev :: t, s) (ev :: nil) (t, s).
 
 Definition atomic : semantics := {|
   state := (trace * state L)%type;
   genvtype := genvtype L;
   step := atomic_step;
-  initial_state := fun s => initial_state L (snd (fst s), snd s) /\ fst (fst s) = E0;
-  final_state := fun s r => final_state L (snd (fst s), snd s) r /\ fst (fst s) = E0;
+  initial_state := fun s => initial_state L (snd s) /\ fst s = E0;
+  final_state := fun s r => final_state L (snd s) r /\ fst s = E0;
   globalenv := globalenv L;
   symbolenv := symbolenv L
 |}.
@@ -1626,13 +1569,13 @@ Variable L2: semantics.
 Context index order match_states (sim: fsim_properties L1 L2 index order match_states).
 Hypothesis L2single: single_events L2.
 
-Inductive ffs_match: index -> meminj -> (trace * state L1 * mem) -> state L2 * mem -> Prop :=
-  | ffs_match_at: forall i f s1 s2 m1,
-      match_states i f (s1,m1) s2 ->
-      ffs_match i f (E0, s1, m1) s2
-  | ffs_match_buffer: forall i f ev t s1 s2 s2' m1,
-      Star L2 s2 (ev :: t) s2' -> match_states i f (s1,m1) s2' ->
-      ffs_match i f (ev :: t, s1, m1) s2.
+Inductive ffs_match: index -> (trace * state L1) -> state L2 -> Prop :=
+  | ffs_match_at: forall i s1 s2,
+      match_states i s1 s2 ->
+      ffs_match i (E0, s1) s2
+  | ffs_match_buffer: forall i ev t s1 s2 s2',
+      Star L2 s2 (ev :: t) s2' -> match_states i s1 s2' ->
+      ffs_match i (ev :: t, s1) s2.
 
 Lemma star_non_E0_split':
   forall s2 t s2', Star L2 s2 t s2' ->
@@ -1652,34 +1595,34 @@ Qed.
 
 Lemma ffs_simulation:
   forall s1 t s1', Step (atomic L1) s1 t s1' ->
-  forall i f s2, ffs_match i f s1 s2 ->
-  exists i', exists s2' f',
+  forall i s2, ffs_match i s1 s2 ->
+  exists i', exists s2',
      (Plus L2 s2 t s2' \/ (Star L2 s2 t s2') /\ order i' i)
-  /\ ffs_match i' f' s1' s2'.
+  /\ ffs_match i' s1' s2'.
 Proof.
   induction 1; intros.
 - (* silent step *)
   inv H0.
   exploit (fsim_simulation sim); eauto.
-  intros [i' [s2' [f' [A B]]]].
-  exists i'; exists s2', f'; split. auto. constructor; auto.
+  intros [i' [s2' [A B]]].
+  exists i'; exists s2'; split. auto. constructor; auto.
 - (* start step *)
   inv H0.
   exploit (fsim_simulation sim); eauto.
-  intros [i' [s2' [f' [A B]]]].
+  intros [i' [s2' [A B]]].
   destruct t as [ | ev' t].
 + (* single event *)
-  exists i'; exists s2', f'; split. auto. constructor; auto.
+  exists i'; exists s2'; split. auto. constructor; auto.
 + (* multiple events *)
   assert (C: Star L2 s2 (ev :: ev' :: t) s2'). intuition. apply plus_star; auto.
   exploit star_non_E0_split'. eauto. simpl. intros [s2x [P Q]].
-  exists i'; exists s2x, f'; split. auto. econstructor; eauto.
+  exists i'; exists s2x; split. auto. econstructor; eauto.
 - (* continue step *)
   inv H0.
   exploit star_non_E0_split'. eauto. simpl. intros [s2x [P Q]].
   destruct t.
-  exists i; exists s2', f; split. left. eapply plus_star_trans; eauto. constructor; auto.
-  exists i; exists s2x, f; split. auto. econstructor; eauto.
+  exists i; exists s2'; split. left. eapply plus_star_trans; eauto. constructor; auto.
+  exists i; exists s2x; split. auto. econstructor; eauto.
 Qed.
 
 End FACTOR_FORWARD_SIMULATION.
@@ -1694,28 +1637,18 @@ Proof.
   apply Forward_simulation with order (ffs_match L1 L2 match_states); constructor.
 - (* wf *)
   eapply fsim_order_wf; eauto.
-- (*Mem.inject *)
-  intros.
-  inversion H; subst.
-  + eapply fsim_match_meminj in H0; eauto.
-  + admit. (*THIS IS FALSE!!!*)
-    (* Now, it is only used in COMPCERT backwards simulation proof, 
-       which we might not need... *)
 - (* initial states *)
   intros. destruct s1 as [t1 s1]. simpl in H. destruct H. subst.
-  exploit (fsim_match_initial_states sim); eauto. intros [i [f [s2 [m2 [A [B MINJ]]]]]].
-  exists i; exists f, s2, m2; split; auto. split; trivial. constructor; auto.
+  exploit (fsim_match_initial_states sim); eauto. intros [i [s2 [A B]]].
+  exists i; exists s2; split; auto. constructor; auto.
 - (* final states *)
   intros. destruct s1 as [t1 s1]. simpl in H0; destruct H0; subst. inv H.
   eapply (fsim_match_final_states sim); eauto.
 - (* simulation *)
-  (*eapply ffs_simulation; eauto.*)
-  intros.
-  destruct (ffs_simulation sim L2single H H0) as [i' [s2' [f' A]]].
-  exists i', s2', f'; trivial.
+  eapply ffs_simulation; eauto.
 - (* symbols preserved *)
   simpl. exact (fsim_public_preserved sim).
-Admitted.
+Qed.
 
 (** Likewise, a backward simulation from a single-event semantics [L1] to a semantics [L2]
   can be "factored" as a backward simulation from [L1] to [atomic L2]. *)
@@ -1727,131 +1660,66 @@ Variable L2: semantics.
 Context index order match_states (sim: bsim_properties L1 L2 index order match_states).
 Hypothesis L1single: single_events L1.
 Hypothesis L2wb: well_behaved_traces L2.
-(*Association (trace * (state L2 * mem)) is more awkward for proving Lemma factor_backward_simulation below.
-  That's why we associate ((trace * state L2) * mem) below
-Inductive fbs_match: index -> meminj -> (state L1 * mem) -> (trace * (state L2 * mem)) -> Prop :=
-  | fbs_match_intro: forall i s1 t s2 s1' f,
-      Star L1 s1 t s1' -> match_states i f s1' s2 ->
+
+Inductive fbs_match: index -> state L1 -> (trace * state L2) -> Prop :=
+  | fbs_match_intro: forall i s1 t s2 s1',
+      Star L1 s1 t s1' -> match_states i s1' s2 ->
       t = E0 \/ output_trace t ->
-      fbs_match i f s1 (t, s2).
+      fbs_match i s1 (t, s2).
 
 Lemma fbs_simulation:
-  forall (s2 :state (atomic L2) * mem) (t : trace) (s2' : state (atomic L2) * mem), 
-  Step (atomic L2) s2 t s2' ->
-  match s2, s2' with ((tr2,ss2),m2), ((tr2',ss2'),m2') =>
-    forall i f s1, fbs_match i f s1 (*s2*)(tr2,(ss2,m2)) -> safe L1 s1 ->
-    exists i' f', exists s1',
-       (Plus L1 s1 t s1' \/ (Star L1 s1 t s1' /\ order i' i))
-       /\ fbs_match i' f' s1' (*s2'*)(tr2',(ss2',m2'))
-  end.
+  forall s2 t s2', Step (atomic L2) s2 t s2' ->
+  forall i s1, fbs_match i s1 s2 -> safe L1 s1 ->
+  exists i', exists s1',
+     (Plus L1 s1 t s1' \/ (Star L1 s1 t s1' /\ order i' i))
+     /\ fbs_match i' s1' s2'.
 Proof.
   induction 1; intros.
 - (* silent step *)
   inv H0.
   exploit (bsim_simulation sim); eauto. eapply star_safe; eauto.
-  intros [i' [f' [s1'' [A B]]]].
-  exists i', f'; exists s1''; split.
+  intros [i' [s1'' [A B]]].
+  exists i'; exists s1''; split.
   destruct A as [P | [P Q]]. left. eapply star_plus_trans; eauto. right; split; auto. eapply star_trans; eauto.
   econstructor. apply star_refl. auto. auto.
 - (* start step *)
   inv H0.
   exploit (bsim_simulation sim); eauto. eapply star_safe; eauto.
-  intros [i' [f' [s1'' [A B]]]].
+  intros [i' [s1'' [A B]]].
   assert (C: Star L1 s1 (ev :: t) s1'').
     eapply star_trans. eauto. destruct A as [P | [P Q]]. apply plus_star; eauto. eauto. auto.
   exploit star_non_E0_split'; eauto. simpl. intros [s1x [P Q]].
-  exists i', f'; exists s1x; split.
+  exists i'; exists s1x; split.
   left; auto.
   econstructor; eauto.
   exploit L2wb; eauto.
 - (* continue step *)
-  inv H0. unfold E0 in (*H8*)H9; destruct (*H8*)H9; try congruence.
+  inv H0. unfold E0 in H8; destruct H8; try congruence.
   exploit star_non_E0_split'; eauto. simpl. intros [s1x [P Q]].
-  exists i, f; exists s1x; split. left; auto. econstructor; eauto. simpl in H0; tauto.
+  exists i; exists s1x; split. left; auto. econstructor; eauto. simpl in H0; tauto.
 Qed.
 
 Lemma fbs_progress:
-  forall i f (s1 : state L1 * mem) (s2 : trace * (state L2 * mem)),
-  fbs_match i f s1 s2 -> safe L1 s1 ->
-  match s2 with (tr2,(ss2,m2)) =>
-    (exists r, final_state (atomic L2) (*s2*) ((tr2,ss2),m2) r) \/
-    (exists t, exists s2', Step (atomic L2) (*s2*) ((tr2,ss2),m2) t s2')
-  end.
+  forall i s1 s2,
+  fbs_match i s1 s2 -> safe L1 s1 ->
+  (exists r, final_state (atomic L2) s2 r) \/
+  (exists t, exists s2', Step (atomic L2) s2 t s2').
 Proof.
-  intros. inv H. destruct s3 as [s3 m3]. destruct t.
+  intros. inv H. destruct t.
 - (* 1. no buffered events *)
   exploit (bsim_progress sim); eauto. eapply star_safe; eauto.
   intros [[r A] | [t [s2' A]]].
 + (* final state *)
   left; exists r; simpl; auto.
 + (* L2 can step *)
-  destruct s2' as [s2' m2']. destruct t. 
-  right; exists E0; exists ((nil, s2'), m2'). constructor. auto.
-  right; exists (e :: nil); exists ((t, s2'), m2'). constructor. auto.
+  destruct t.
+  right; exists E0; exists (nil, s2'). constructor. auto.
+  right; exists (e :: nil); exists (t, s2'). constructor. auto.
 - (* 2. some buffered events *)
   unfold E0 in H3; destruct H3. congruence.
-  right; exists (e :: nil); exists ((t, s3), m3). constructor. auto.
-Qed.
-*)
-Inductive fbs_match: index -> meminj -> (state L1 * mem) -> ((trace * state L2) * mem) -> Prop :=
-  | fbs_match_intro: forall i s1 t s2 m2 s1' f,
-      Star L1 s1 t s1' -> match_states i f s1' (s2,m2) ->
-      t = E0 \/ output_trace t ->
-      fbs_match i f s1 ((t, s2),m2).
-
-Lemma fbs_simulation:
-  forall (s2 :state (atomic L2) * mem) (t : trace) (s2' : state (atomic L2) * mem), 
-  Step (atomic L2) s2 t s2' ->
-    forall i f s1, fbs_match i f s1 s2 -> safe L1 s1 ->
-    exists i' f', exists s1',
-       (Plus L1 s1 t s1' \/ (Star L1 s1 t s1' /\ order i' i))
-       /\ fbs_match i' f' s1' s2'.
-Proof.
-  induction 1; intros.
-- (* silent step *)
-  inv H0.
-  exploit (bsim_simulation sim); eauto. eapply star_safe; eauto.
-  intros [i' [f' [s1'' [A B]]]].
-  exists i', f'; exists s1''; split.
-  destruct A as [P | [P Q]]. left. eapply star_plus_trans; eauto. right; split; auto. eapply star_trans; eauto.
-  econstructor. apply star_refl. auto. auto.
-- (* start step *)
-  inv H0.
-  exploit (bsim_simulation sim); eauto. eapply star_safe; eauto.
-  intros [i' [f' [s1'' [A B]]]].
-  assert (C: Star L1 s1 (ev :: t) s1'').
-    eapply star_trans. eauto. destruct A as [P | [P Q]]. apply plus_star; eauto. eauto. auto.
-  exploit star_non_E0_split'; eauto. simpl. intros [s1x [P Q]].
-  exists i', f'; exists s1x; split.
-  left; auto.
-  econstructor; eauto.
-  exploit L2wb; eauto.
-- (* continue step *)
-  inv H0. unfold E0 in (*H8*)H10; destruct (*H8*)H10; try congruence.
-  exploit star_non_E0_split'; eauto. simpl. intros [s1x [P Q]].
-  exists i, f; exists s1x; split. left; auto. econstructor; eauto. simpl in H0; tauto.
+  right; exists (e :: nil); exists (t, s3). constructor. auto.
 Qed.
 
-Lemma fbs_progress:
-  forall i f (s1 : state L1 * mem) (s2 : (trace * state L2) * mem),
-  fbs_match i f s1 s2 -> safe L1 s1 ->
-    (exists r, final_state (atomic L2) s2 r) \/
-    (exists t, exists s2', Step (atomic L2) s2 t s2').
-Proof.
-  intros. inv H. rename m2 into m3. destruct t.
-- (* 1. no buffered events *)
-  exploit (bsim_progress sim); eauto. eapply star_safe; eauto.
-  intros [[r A] | [t [s2' A]]].
-+ (* final state *)
-  left; exists r; simpl; auto.
-+ (* L2 can step *)
-  destruct s2' as [s2' m2']. destruct t. 
-  right; exists E0; exists ((nil, s2'), m2'). constructor. auto.
-  right; exists (e :: nil); exists ((t, s2'), m2'). constructor. auto.
-- (* 2. some buffered events *)
-  unfold E0 in H3; destruct H3. congruence.
-  right; exists (e :: nil); exists ((t, s3), m3). constructor. auto.
-Qed.
 End FACTOR_BACKWARD_SIMULATION.
 
 Theorem factor_backward_simulation:
@@ -1865,25 +1733,20 @@ Proof.
 - (* wf *)
   eapply bsim_order_wf; eauto.
 - (* initial states exist *)
-  intros. exploit (bsim_initial_states_exist sim); eauto. intros [[s2 m2] A].
-  exists ((E0, s2),m2). simpl; auto.
+  intros. exploit (bsim_initial_states_exist sim); eauto. intros [s2 A].
+  exists (E0, s2). simpl; auto.
 - (* initial states match *)
-  intros. destruct s2 as [[t s2] m2]; simpl in H0; destruct H0; subst.
-  exploit (bsim_match_initial_states sim); eauto. intros [i [s1' [f [A [B MINJ]]]]].
-  exists i; exists s1'; exists f; split. auto. split. econstructor. apply star_refl. auto. auto. trivial.
+  intros. destruct s2 as [t s2]; simpl in H0; destruct H0; subst.
+  exploit (bsim_match_initial_states sim); eauto. intros [i [s1' [A B]]].
+  exists i; exists s1'; split. auto. econstructor. apply star_refl. auto. auto.
 - (* final states match *)
-  intros. destruct s2 as [[t s2] m2]; simpl in H1; destruct H1; subst.
+  intros. destruct s2 as [t s2]; simpl in H1; destruct H1; subst.
   inv H. exploit (bsim_match_final_states sim); eauto. eapply star_safe; eauto.
   intros [s1'' [A B]]. exists s1''; split; auto. eapply star_trans; eauto.
 - (* progress *)
-  (*eapply fbs_progress; eauto.*)
-  intros. destruct (fbs_progress sim H H0). 
-  + left; trivial.
-  + right. destruct H1 as [tr [s2' A]]. exists tr, s2'. trivial.
+  eapply fbs_progress; eauto.
 - (* simulation *)
-  (*eapply fbs_simulation; eauto.*)
-  intros. destruct (fbs_simulation sim L1single L2wb H H0 H1) as [i' [f' [s1' A]]].
-  exists i', f', s1'; trivial.
+  eapply fbs_simulation; eauto.
 - (* symbols *)
   simpl. exact (bsim_public_preserved sim).
 Qed.
@@ -1904,23 +1767,22 @@ Theorem atomic_receptive:
   forall L, strongly_receptive L -> receptive (atomic L).
 Proof.
   intros. constructor; intros.
-- (* receptive *)
+(* receptive *)
   inv H0.
-+ (* silent step *)
-  inv H1. exists ((E0, s'),m'). constructor; auto.
+  (* silent step *)
+  inv H1. exists (E0, s'). constructor; auto.
   (* start step *)
-+ assert (exists ev2, t2 = ev2 :: nil). inv H1; econstructor; eauto.
+  assert (exists ev2, t2 = ev2 :: nil). inv H1; econstructor; eauto.
   destruct H0 as [ev2 EQ]; subst t2.
   exploit ssr_receptive; eauto. intros [s2 [t2 P]].
   exploit ssr_well_behaved. eauto. eexact P. simpl; intros Q.
-  destruct s2 as [s2 m2].
-  exists ((t2, s2),m2). constructor; auto.
+  exists (t2, s2). constructor; auto.
   (* continue step *)
-+ simpl in H2; destruct H2.
+  simpl in H2; destruct H2.
   assert (t2 = ev :: nil). inv H1; simpl in H0; tauto.
-  subst t2. exists ((t, s0), m). constructor; auto. simpl; auto.
+  subst t2. exists (t, s0). constructor; auto. simpl; auto.
 (* single-event *)
-- red. intros. inv H0; simpl; omega.
+  red. intros. inv H0; simpl; omega.
 Qed.
 
 (** * Connections with big-step semantics *)
